Foundation/Modal/Kripke/Completeness.lean
@@ -10,20 +10,20 @@ open MaximalConsistentTheory
 open Hilbert.Deduction
 
 variable {α : Type u} [DecidableEq α]
-variable {Λ : Hilbert α} [Λ.IsNormal]
+variable {H : Hilbert α} [H.IsNormal]
 
 namespace Kripke
 
-abbrev CanonicalFrame (Λ : Hilbert α) [Nonempty (MCT Λ)] : Kripke.Frame where
-  World := MCT Λ
+abbrev CanonicalFrame (H : Hilbert α) [Nonempty (MCT H)] : Kripke.Frame where
+  World := MCT H
   Rel Ω₁ Ω₂ := □''⁻¹Ω₁.theory ⊆ Ω₂.theory
 
 namespace CanonicalFrame
 
-variable [Nonempty (MCT Λ)]
-variable {Ω₁ Ω₂ : (CanonicalFrame Λ).World}
+variable [Nonempty (MCT H)]
+variable {Ω₁ Ω₂ : (CanonicalFrame H).World}
 
-omit [DecidableEq α] [Λ.IsNormal] in
+omit [DecidableEq α] [H.IsNormal] in
 @[simp] lemma rel_def_box: Ω₁ ≺ Ω₂ ↔ ∀ {φ}, □φ ∈ Ω₁.theory → φ ∈ Ω₂.theory := by simp [Frame.Rel']; aesop;
 
 lemma multirel_def_multibox : Ω₁ ≺^[n] Ω₂ ↔ ∀ {φ}, □^[n]φ ∈ Ω₁.theory → φ ∈ Ω₂.theory := by
@@ -39,12 +39,12 @@ lemma multirel_def_multibox : Ω₁ ≺^[n] Ω₂ ↔ ∀ {φ}, □^[n]φ ∈ Ω
       obtain ⟨⟨Ω₃, _⟩, R₁₃, R₃₂⟩ := h;
       apply ih.mp R₃₂ $ rel_def_box.mp R₁₃ (by simpa using hp);
     . intro h;
-      obtain ⟨Ω, hΩ⟩ := lindenbaum (Λ := Λ) (T := (□''⁻¹Ω₁.theory ∪ ◇''^[n]Ω₂.theory)) $ by
+      obtain ⟨Ω, hΩ⟩ := lindenbaum (H := H) (T := (□''⁻¹Ω₁.theory ∪ ◇''^[n]Ω₂.theory)) $ by
         apply Theory.intro_union_consistent;
         rintro Γ Δ ⟨hΓ, hΔ⟩ hC;
 
         replace hΓ : ∀ φ ∈ Γ, □φ ∈ Ω₁.theory := by simpa using hΓ;
-        have dΓconj : Ω₁.theory *⊢[Λ]! □⋀Γ := membership_iff.mp $ iff_mem_box_conj.mpr hΓ;
+        have dΓconj : Ω₁.theory *⊢[H]! □⋀Γ := membership_iff.mp $ iff_mem_box_conj.mpr hΓ;
 
         have hΔ₂ : ∀ φ ∈ ◇'⁻¹^[n]Δ, φ ∈ Ω₂.theory := by
           intro φ hp;
@@ -53,19 +53,19 @@ lemma multirel_def_multibox : Ω₁ ≺^[n] Ω₂ ↔ ∀ {φ}, □^[n]φ ∈ Ω
         have hΔconj : ⋀◇'⁻¹^[n]Δ ∈ Ω₂.theory := iff_mem_conj.mpr hΔ₂;
 
         have : ⋀◇'⁻¹^[n]Δ ∉ Ω₂.theory := by {
-          have d₁ : Λ ⊢! ⋀Γ ➝ ⋀Δ ➝ ⊥ := and_imply_iff_imply_imply'!.mp hC;
-          have : Λ ⊢! ⋀(◇'^[n]◇'⁻¹^[n]Δ) ➝ ⋀Δ := by
+          have d₁ : H ⊢! ⋀Γ ➝ ⋀Δ ➝ ⊥ := and_imply_iff_imply_imply'!.mp hC;
+          have : H ⊢! ⋀(◇'^[n]◇'⁻¹^[n]Δ) ➝ ⋀Δ := by
             apply conjconj_subset!;
             intro ψ hq;
             obtain ⟨χ, _, _⟩ := hΔ ψ hq;
             subst_vars;
             simpa;
-          have : Λ ⊢! ◇^[n]⋀◇'⁻¹^[n]Δ ➝ ⋀Δ := imp_trans''! iff_conjmultidia_multidiaconj! $ this;
-          have : Λ ⊢! ∼(□^[n](∼⋀◇'⁻¹^[n]Δ)) ➝ ⋀Δ := imp_trans''! (and₂'! multidia_duality!) this;
-          have : Λ ⊢! ∼⋀Δ ➝ □^[n](∼⋀◇'⁻¹^[n]Δ) := contra₂'! this;
-          have : Λ ⊢! (⋀Δ ➝ ⊥) ➝ □^[n](∼⋀◇'⁻¹^[n]Δ) := imp_trans''! (and₂'! neg_equiv!) this;
-          have : Λ ⊢! ⋀Γ ➝ □^[n](∼⋀◇'⁻¹^[n]Δ) := imp_trans''! d₁ this;
-          have : Λ ⊢! □⋀Γ ➝ □^[(n + 1)](∼⋀◇'⁻¹^[n]Δ) := by simpa using imply_box_distribute'! this;
+          have : H ⊢! ◇^[n]⋀◇'⁻¹^[n]Δ ➝ ⋀Δ := imp_trans''! iff_conjmultidia_multidiaconj! $ this;
+          have : H ⊢! ∼(□^[n](∼⋀◇'⁻¹^[n]Δ)) ➝ ⋀Δ := imp_trans''! (and₂'! multidia_duality!) this;
+          have : H ⊢! ∼⋀Δ ➝ □^[n](∼⋀◇'⁻¹^[n]Δ) := contra₂'! this;
+          have : H ⊢! (⋀Δ ➝ ⊥) ➝ □^[n](∼⋀◇'⁻¹^[n]Δ) := imp_trans''! (and₂'! neg_equiv!) this;
+          have : H ⊢! ⋀Γ ➝ □^[n](∼⋀◇'⁻¹^[n]Δ) := imp_trans''! d₁ this;
+          have : H ⊢! □⋀Γ ➝ □^[(n + 1)](∼⋀◇'⁻¹^[n]Δ) := by simpa using imply_box_distribute'! this;
           exact iff_mem_neg.mp $ h $ membership_iff.mpr $ (Context.of! this) ⨀ dΓconj;
         }
 
@@ -93,17 +93,17 @@ lemma rel_def_dia : Ω₁ ≺ Ω₂ ↔ ∀ {φ}, φ ∈ Ω₂.theory → ◇φ 
 end CanonicalFrame
 
 
-abbrev CanonicalModel (Λ : Hilbert α) [Nonempty (MCT Λ)]  : Model α where
-  Frame := CanonicalFrame Λ
+abbrev CanonicalModel (H : Hilbert α) [Nonempty (MCT H)]  : Model α where
+  Frame := CanonicalFrame H
   Valuation Ω a := (atom a) ∈ Ω.theory
 
 
 namespace CanonicalModel
 
-variable [Nonempty (MCT Λ)]
+variable [Nonempty (MCT H)]
 
 @[reducible]
-instance : Semantics (Formula α) (CanonicalModel Λ).World := Formula.Kripke.Satisfies.semantics (M := CanonicalModel Λ)
+instance : Semantics (Formula α) (CanonicalModel H).World := Formula.Kripke.Satisfies.semantics (M := CanonicalModel H)
 
 -- @[simp] lemma frame_def : (CanonicalModel Ax).Rel' Ω₁ Ω₂ ↔ (□''⁻¹Ω₁.theory : Theory α) ⊆ Ω₂.theory := by rfl
 -- @[simp] lemma val_def : (CanonicalModel Ax).Valuation Ω a ↔ (atom a) ∈ Ω.theory := by rfl
@@ -113,9 +113,9 @@ end CanonicalModel
 
 section
 
-variable [Nonempty (MCT Λ)] {φ : Formula α}
+variable [Nonempty (MCT H)] {φ : Formula α}
 
-lemma truthlemma : ∀ {Ω : (CanonicalModel Λ).World}, Ω ⊧ φ ↔ (φ ∈ Ω.theory) := by
+lemma truthlemma : ∀ {Ω : (CanonicalModel H).World}, Ω ⊧ φ ↔ (φ ∈ Ω.theory) := by
   induction φ using Formula.rec' with
   | hbox φ ih =>
     intro Ω;
@@ -144,15 +144,15 @@ lemma truthlemma : ∀ {Ω : (CanonicalModel Λ).World}, Ω ⊧ φ ↔ (φ ∈ �
   | _ => simp_all [Kripke.Satisfies];
 
 
-lemma iff_valid_on_canonicalModel_deducible : (CanonicalModel Λ) ⊧ φ ↔ Λ ⊢! φ := by
+lemma iff_valid_on_canonicalModel_deducible : (CanonicalModel H) ⊧ φ ↔ H ⊢! φ := by
   constructor;
   . contrapose;
     intro h;
-    have : Theory.Consistent Λ ({∼φ}) := by
+    have : Theory.Consistent H ({∼φ}) := by
       apply Theory.def_consistent.mpr;
       intro Γ hΓ;
       by_contra hC;
-      have : Λ ⊢! φ := dne'! $ neg_equiv'!.mpr $ replace_imply_left_conj! hΓ hC;
+      have : H ⊢! φ := dne'! $ neg_equiv'!.mpr $ replace_imply_left_conj! hΓ hC;
       contradiction;
     obtain ⟨Ω, hΩ⟩ := lindenbaum this;
     simp [Kripke.ValidOnModel];
@@ -162,17 +162,17 @@ lemma iff_valid_on_canonicalModel_deducible : (CanonicalModel Λ) ⊧ φ ↔ Λ 
     suffices φ ∈ Ω.theory by exact truthlemma.mpr this;
     by_contra hC;
     obtain ⟨Γ, hΓ₁, hΓ₂⟩ := Theory.iff_insert_inconsistent.mp $ (MaximalConsistentTheory.maximal' hC);
-    have : Γ ⊢[Λ]! ⊥ := FiniteContext.provable_iff.mpr $ and_imply_iff_imply_imply'!.mp hΓ₂ ⨀ h;
-    have : Γ ⊬[Λ] ⊥ := Theory.def_consistent.mp Ω.consistent _ hΓ₁;
+    have : Γ ⊢[H]! ⊥ := FiniteContext.provable_iff.mpr $ and_imply_iff_imply_imply'!.mp hΓ₂ ⨀ h;
+    have : Γ ⊬[H] ⊥ := Theory.def_consistent.mp Ω.consistent _ hΓ₁;
     contradiction;
 
-lemma realize_axiomset_of_self_canonicalModel : (CanonicalModel Λ) ⊧* Λ.axioms := by
+lemma realize_axiomset_of_self_canonicalModel : (CanonicalModel H) ⊧* H.axioms := by
   apply Semantics.realizeSet_iff.mpr;
   intro φ hp;
   apply iff_valid_on_canonicalModel_deducible.mpr;
   exact maxm! hp;
 
-lemma realize_theory_of_self_canonicalModel : (CanonicalModel Λ) ⊧* (System.theory Λ) := by
+lemma realize_theory_of_self_canonicalModel : (CanonicalModel H) ⊧* (System.theory H) := by
   apply Semantics.realizeSet_iff.mpr;
   intro φ hp;
   apply iff_valid_on_canonicalModel_deducible.mpr;
@@ -180,18 +180,18 @@ lemma realize_theory_of_self_canonicalModel : (CanonicalModel Λ) ⊧* (System.t
 
 end
 
-lemma complete_of_mem_canonicalFrame [Nonempty (MCT Λ)] {𝔽 : FrameClass} (hFC : CanonicalFrame Λ ∈ 𝔽) : 𝔽#α ⊧ φ → (Λ) ⊢! φ := by
+lemma complete_of_mem_canonicalFrame [Nonempty (MCT H)] {𝔽 : FrameClass} (hFC : CanonicalFrame H ∈ 𝔽) : 𝔽#α ⊧ φ → (H) ⊢! φ := by
   simp [Semantics.Realize, Kripke.ValidOnFrame];
   contrapose;
   push_neg;
   intro h;
-  use (CanonicalFrame Λ);
+  use (CanonicalFrame H);
   constructor;
   . assumption;
-  . use (CanonicalModel Λ).Valuation;
+  . use (CanonicalModel H).Valuation;
     exact iff_valid_on_canonicalModel_deducible.not.mpr h;
 
-instance instComplete_of_mem_canonicalFrame [Nonempty (MCT Λ)] (𝔽 : FrameClass) (hFC : CanonicalFrame Λ ∈ 𝔽) : Complete (Λ) (𝔽#α) := ⟨complete_of_mem_canonicalFrame hFC⟩
+instance instComplete_of_mem_canonicalFrame [Nonempty (MCT H)] (𝔽 : FrameClass) (hFC : CanonicalFrame H ∈ 𝔽) : Complete (H) (𝔽#α) := ⟨complete_of_mem_canonicalFrame hFC⟩
 
 instance K_complete : Complete (Hilbert.K α) (AllFrameClass.{u}#α) := by
   convert instComplete_of_mem_canonicalFrame (α := α) AllFrameClass trivial;
